# Предел функции.

## Найти предел функции:

1. $$\lim\limits_{x \to \infty}\frac{(23 - 2x^2)(3x^2 + 17)^2}{4x^6 + x - 1} = \left({\color{red}{\frac{\infty}{\infty}}}\right) = $$

$$\lim\limits_{x \to \infty}\frac{(23 - 2x^2)(3x^2 + 17)(3x^2 + 17)}{4x^6 + x - 1} = \lim\limits_{x \to \infty}\frac{(23 - 2x^2)(9x^4 + 102x^2 + 289)}{4x^6 + x - 1} = $$

$$\lim\limits_{x \to \infty}\frac{-18x^6 +3x^4+1768x^2 + 6647}{4x^6 + x - 1} = \frac{-18}{4} = -\frac{9}{2} = -4 \frac{1}{2}$$

2. $$\lim\limits_{x \to \infty}\frac{(97 - 2x)^3}{2x(3x^2 +15) + 8x} = \left({\color{red}{\frac{\infty}{\infty}}}\right) =$$

$$\lim\limits_{x \to \infty}\frac{-8x^3 + 1164x^2  - 56454x + 912673}{6x^3 + 38x} = \frac{-8}{6} = -\frac{4}{3} = -1\frac{1}{3}$$

3. $$\lim\limits_{x \to \infty}\frac{2x^3 + 13x(x +18)}{(27 - x)(2x + 19)^2} = \left({\color{red}{\frac{\infty}{\infty}}}\right) = $$

$$\lim\limits_{x \to \infty}\frac{2x^3 + 13x^2 + 234x}{(27 - x)(2x + 19)(2x + 19)} = \lim\limits_{x \to \infty}\frac{2x^3 + 13x^2 + 234x}{-4x^3 + 32x^2 + 1691x +9747} = \frac{2}{-4} = -\frac{1}{2}$$

4. $$\lim\limits_{x \to 6}\frac{x^2 - 36}{x^2 - x - 30} = \left({\color{red}{\frac{0}{0}}}\right) =$$

$$\lim\limits_{x \to 6}\frac{(x - 6)(x + 6)}{(x - 6)(x + 5)} = \lim\limits_{x \to 6}\frac{x + 6}{x + 5} = \frac{12}{11} = 1\frac{1}{11}$$

5. $$\lim\limits_{x \to 7}\frac{x^2 - 49}{x^2 - 13x + 42} = \left({\color{red}{\frac{0}{0}}}\right) = $$

$$\lim\limits_{x \to 7}\frac{(x - 7)(x + 7)}{(x - 7)(x - 6)} = \lim\limits_{x \to 7}\frac{x + 7}{x - 6} = \frac{14}{1} = 14$$

6. \* $$\lim\limits_{x \to 7}\frac{\sqrt{x + 2} - \sqrt[3]{x + 20}}{\sqrt[4]{x + 9} - 2} =\frac
{112}{27}$$

7. $$\lim\limits_{x \to 0}\frac{3x\tan{4x}}{1 - \cos{4x}} = \left({\color{red}{\frac{0}{0}}}\right) =$$

$$ \lim\limits_{x \to 0}\frac{3x\tan{4x}}{1 - \cos{4x}} \cdot \frac{4x}{4x} \cdot \frac{\frac{(4x)^2}{2}}{\frac{(4x)^2}{2}}= \frac{3x \cdot 1 \cdot 4x \cdot 2}{16x^2} = \frac{24x^2}{16x^2} = \frac{3}{2} = 1\frac{1}{2}$$

8. \*\* $$\lim\limits_{x \to 0}\frac{\sqrt{2}x^2\sin{4x}}{(1 - \cos{2x})^{\frac{3}{2}}} = \lim\limits_{x \to 0}\frac{\sqrt{2}x^2\sin{4x}}{(2\sin^2{x})^{\frac{3}{2}}} = \lim\limits_{x \to 0}\frac{\sqrt{2}x^2\cdot{4x}}{2^{\frac{3}{2}}\cdot |x|^3} =\pm 2$$

9. $$\lim\limits_{x \to \infty}\left(\frac{4x}{4x + 3}\right)^{\frac{5x^2}{7x - 1}} = \left({\color{red}{\frac{\infty}{\infty}}}\right) = $$

$$\lim\limits_{x \to \infty}\left(1 + \frac{3}{4x + 3}\right)^{\frac{5x^2}{7x - 1}} = ({\color{red}{e^\infty}}) = $$

$$\lim\limits_{x \to \infty}\left(1 + \frac{3}{4x + 3}\right)^{\frac{5x^2}{7x - 1} \cdot \frac{4x + 3}{3} \cdot \frac{3}{4x + 3}} = $$

$$e^{\lim\limits_{x \to \infty}\frac{5x^2}{7x - 1} \cdot \frac{3}{4x + 3}} = e^{\lim\limits_{x \to \infty}\frac{15x^2}{28x^2 + 17x - 3}} = e^{\frac{15}{28}}$$

10. \* $$\lim\limits_{x \to \infty}\frac{\ln{(x^2 - x + 1)}}{\ln{(x^{10} + x + 1)}} = \lim\limits_{x \to \infty}\frac{\ln{x^2}+\ln{(1 - \frac{1}{x} + \frac{1}{x^2})}}{\ln{x^{10}} + \ln{(1 + \frac{1}{x^9} + \frac{1}{x^{10}})}} = \lim\limits_{x \to \infty}\frac{2\ln{|x|}}{10\ln{|x|}} = \frac{2}{10} = \frac{1}{5}$$

11. $$\lim\limits_{x \to 0}\frac{5^x - 1}{x} = \left({\color{red}{\frac{0}{0}}}\right) = $$

$$\lim\limits_{x \to 0}\frac{\frac{d}{dx}[5^x - 1]}{\frac{d}{dx}[x]} = \lim\limits_{x \to 0}\frac{5^x \ln{5}}{1} = \ln{5} $$
